examples/Queue/queue_mli.v
@@ -38,8 +38,23 @@ Module Declarations.
   Class _create__spec_sig `{@_create__sig} `{@_T_sig}  := {
     create__spec :
       forall {A}, forall `{Enc A}, forall `{Inhab A}, SPEC(create_  tt )
-      PRE \[]
+      PRE( \[] )
       POST(fun q_ : t_ A=> q_ ~> T empty )
+  }.
+
+  Class _add__sig  := { add_ : val }.
+
+  Class _add__spec_sig `{@_add__sig} `{@_T_sig}  := {
+    add__spec :
+      forall {A}, forall `{Enc A}, forall
+      `{Inhab A}
+      (x_ : A)
+      (x : val)
+      (q_ : t_ A)
+      (q : sequence val),
+      SPEC(add_  x_ q_ )
+      PRE( x_ ~> Val x\*q_ ~> T q )
+      POSTUNIT( x_ ~> Val x\*q_ ~> T (snoc q x) )
   }.
 
 End Declarations.
@@ -59,5 +74,13 @@ Module Type Obligations.
   (* Separation Logic Triple create__spec *)
 
   Global Declare Instance _create__spec_inst : _create__spec_sig.
+
+  (* Program Value add_ *)
+
+  Global Declare Instance _add__inst : _add__sig.
+
+  (* Separation Logic Triple add__spec *)
+
+  Global Declare Instance _add__spec_inst : _add__spec_sig.
 
 End Obligations.
