examples/Queue/queue_proof.v
@@ -1,3 +1,4 @@
+Set Implicit Arguments.
 Require Import Gospel.CFML.base queue_ml queue_mli.
 
 From EXAMPLES Require Primitives.
@@ -9,16 +10,10 @@ Require Import
   Stdlib.ZArith.BinIntDef
   Stdlib.Strings.Ascii.
 
-Require Import
-  CFML.SepBase
-  CFML.SepLifted
-  CFML.WPLib
-  CFML.WPLifted
-  CFML.WPRecord
-  CFML.WPArray
-  CFML.WPBuiltin
-  CFML.Semantics
-  CFML.WPHeader.
+From CFML Require Import Stdlib.
+
+From CFML Require Import WPLib.
+From CFML Require Import Stdlib.
 
 Module Proofs : Obligations.
 
@@ -26,27 +21,127 @@ Module Proofs : Obligations.
 
   Import queue_ml.
 
-  Declare Instance Enc_cell_ (A : Type) : Enc (cell_ A).
+  Definition Cell A `{Enc A} (x : val) (next c : cell_ A) :=
+    \exists (l: loc) (v : A),
+      \[c = Cons l] \* \[x = ``v] \* l ~~~> `{ content' := v; next' := next }.
 
-  Hint Constructors cell_ : typeclass_instances.
+  Lemma Cell_eq :
+    forall A (E : Enc A) l (c : A) (n :  cell_ A),
+      l ~~~> `{ content' := c; next' := n } = Cons l ~> Cell ``c n.
+  Proof.
+    intros A E l c n.
+    xunfold Cell. xsimpl l c. 1, 2: auto.
+    intros x v [= H1] H2.
+    subst. xsimpl. apply enc_inj in H2. auto.
+  Qed.
 
-  Global Instance _T_inst : _T_sig :=
-    { T := fun A _ (m : list val) l =>
-             match m with
-             |nil => l ~> Record `{length' := 0; first' := Nil; last' := Nil}
-             |_ => \[True] end}.
+  Fixpoint Cell_seg A `{Enc A} (l : list val) (e : cell_ A) (st : cell_ A) :=
+    match l with
+    |nil => \[st = e]
+    |cons x l =>
+       \exists n : cell_ A, st ~> Cell x n \* n ~> Cell_seg l e
+    end.
+
+  Lemma Cell_seg_nil : forall A (EA: Enc A) (to from: cell_ A),
+      from ~> Cell_seg (@nil val) to = \[from = to].
+  Proof using. auto. Qed.
+
+  Definition single_seg :
+    forall A `{Enc A} (x : val) cell,
+      cell ~> Cell (A:=A) x Nil = Cell_seg (x :: nil) Nil cell.
+  Proof.
+    intros A H x cell.
+    xpull.
+    + xunfold Cell_seg. xsimpl. rewrite <- Cell_seg_nil.
+    + xunfold Cell_seg. xpull.
+      intros.
+
+  Admitted.
+
+  Import LibListZ.
+
+  Definition Queue A `{Enc A} (l : list val) (q : loc) :=
+    \exists (cf cl: cell_ A),
+           (q ~~~> `{ length' := LibListZ.length l; first' := cf; last' := cl }) \*
+             If l = nil then \[cf = Nil] \* \[cl = Nil]
+  else
+    \exists L x,
+      \[l = L & x] \*
+            cf ~> Cell_seg L cl \* cl ~> Cell_seg (x::nil) Nil.
+
+  Definition Queue_if A `{Enc A} (l : list val) (q : loc) :=
+    \exists (cf cl : cell_ A),
+      (q ~~~> `{ length' := LibListZ.length l; first' := cf; last' := cl }) \*
+      If cl = Nil then \[cl = Nil] \* \[l = nil]
+  else
+    \exists L x,
+      \[l = L & x] \*
+         cf ~> Cell_seg L cl \* cl ~> Cell_seg (x::nil) Nil.
+
+  Lemma Queue_inv : forall A (E : Enc A) l q, q ~> @Queue A E l ==> q ~> @Queue_if A E l.
+    intros A E l q.
+    xunfold* Queue. xpull ;=> cf cl.
+    case_if.
+    + xsimpl ;=> -> ->.
+      xunfold Queue_if. xsimpl. case_if; xsimpl; auto.
+    + xsimpl ;=> x t H1. subst.
+      xunfold Queue_if.
+      xsimpl. case_if.
+      - subst. xunfold Cell_seg. xunfold Cell. xsimpl.
+      - xsimpl. auto.
+  Qed.
+
+  Global Instance _T_inst : _T_sig := {
+      T := Queue
+  }.
 
   Global Instance _create__inst : _create__sig :=
     { create_ := create }.
 
   #[refine] Global Instance _create__spec_inst : _create__spec_sig := { }.
   Proof.
-    intros.
+    intros A Enc _.
     simpl.
     xcf.
-    applys xapp_lemma_record_new.
+    xapp.
+    xunfold Queue.
     intros.
+    rew_list.
     xsimpl.
+    case_if.
+    xsimpl; auto.
+  Qed.
 
+  Global Instance _add__inst : _add__sig :=
+    { add_ := add }.
+
+  Set Implicit Arguments.
+
+  #[refine] Global Instance _add__spec_inst : _add__spec_sig := { }.
+  Proof.
+    simpl.
+    intros A E _ x'' x q'' q.
+    xcf. xunfold (@Primitives.Val A). xpull. intros. subst.
+    xapp ;=> cell.
+    xlet. subst.
+    xchanges Queue_inv.
+    xunfold Queue_if.
+    xpull ;=> cf ce.
+    destruct q; case_if.
+    + xpull ;=> H1 _.
+      xapp. xmatch. do 3 xapp.
+      xsimpl*. rew_list.
+      xsimpl. xchange Cell_eq. xchange single_seg.
+      xunfold Queue. xsimpl (@Cons A cell) (@Cons A cell).
+      case_if. xsimpl (@nil val) ``x''. rew_list. auto.
+      xunfold Cell_seg. xsimpl*.
+    + xpull ;=> L x H1. Search app.
+      apply nil_eq_app_inv in H1 as [_ H2].
+      inversion H2.
+    + xpull.
+    + xpull ;=> L x H1. xapp.
+      xmatch. xapp. xapp.
+
+   Admitted.
 
 End Proofs.
